Filled admits + var sets + unification by steps + existence of unification result

Unify.v
@@ -2,10 +2,16 @@ Require Import List.
 Import ListNotations.
 Require Import Arith.
 Require Import Omega.
+Require Import Coq.Lists.ListSet.
+Require Export Coq.Structures.OrderedTypeEx.
+Require Import Eqdep.
+Require Import Program.
 
 (************************* Terms *************************)
 (* Name of entities *)
 Definition name := nat.
+
+Definition name_eq_dec : (forall x y : name, {x = y} + {x <> y}) := eq_nat_dec.
 
 (* Term type *) 
 Inductive term : Set :=
@@ -13,20 +19,54 @@ Inductive term : Set :=
 (* a constant           *) | Cst : name -> term
 (* a binary constructor *) | Con : name -> term -> term -> term.
 
-Fixpoint fv_term (t : term) : list name :=
+Definition var_set := set name.
+
+Definition var_set_empty : var_set := empty_set name.
+Definition var_set_add : name -> var_set -> var_set := set_add name_eq_dec.
+Definition var_set_union : var_set -> var_set -> var_set := set_union name_eq_dec.
+Definition var_set_remove : name -> var_set -> var_set := set_remove name_eq_dec.
+Definition var_set_size : var_set -> nat := @length name.
+
+Fixpoint fv_term (t : term) : var_set :=
   match t with
-  | Var n     => [n]
-  | Cst _     => []
-  | Con _ l r => fv_term l ++ fv_term r
+  | Var n     => var_set_add n var_set_empty
+  | Cst _     => var_set_empty
+  | Con _ l r => var_set_union (fv_term l) (fv_term r)
   end.
 
-Definition fv_terms (ts : list term) : list name :=
-  fold_left (fun acc t => acc ++ fv_term t) ts [].
+Lemma fv_term_nodup : forall t, NoDup (fv_term t).
+Proof.
+  induction t.
+  * apply set_add_nodup. constructor.
+  * constructor.
+  * apply set_union_nodup; assumption.
+Qed.
+
+Definition fv_terms (ts : list term) : var_set :=
+  fold_left (fun acc t => var_set_union acc (fv_term t)) ts var_set_empty.
 
 Lemma free_var (t : term) : exists x, ~ In x (fv_term t).
 Proof.
-  admit.
-Admitted.
+  assert (A : forall t, exists n, forall x, In x (fv_term t) -> S x <= n).
+  {
+    clear. induction t.
+    * exists (S n). intros. destruct H.
+      + omega.
+      + contradiction.
+    * exists 0. intros. contradiction.
+    * destruct IHt1 as [n1 IHt1]. destruct IHt2 as [n2 IHt2].
+      exists (max n1 n2). intros. apply (set_union_elim name_eq_dec) in H.
+      destruct H.
+      + eapply le_trans.
+        - eapply IHt1. assumption.
+        - apply Nat.le_max_l.
+      + eapply le_trans.
+        - eapply IHt2. assumption.
+        - apply Nat.le_max_r.
+  }
+  specialize (A t). destruct A. exists x. intro C.
+  apply H in C. omega.
+Qed.
 
 Fixpoint height (t : term) : nat :=
   match t with
@@ -42,6 +82,26 @@ Fixpoint occurs (n : name) (t : term) : bool :=
   | Con _ l r => orb (occurs n l) (occurs n r)
   end.
 
+Lemma occurs_In: forall t n, occurs n t = true <-> In n (fv_term t).
+Proof.
+  intros. induction t.
+  * split; intro.
+    + left. symmetry. apply Nat.eqb_eq. assumption.
+    + destruct H.
+      - apply Nat.eqb_eq. symmetry. assumption.
+      - contradiction.
+  * split; intro C; inversion C.
+  * split; intro.
+    + apply (set_union_intro name_eq_dec).
+      apply Bool.orb_true_elim in H. destruct H.
+      - left. apply IHt1. assumption.
+      - right. apply IHt2. assumption.
+    + apply Bool.orb_true_intro.
+      apply (set_union_elim name_eq_dec) in H. destruct H.
+      - left. apply IHt1. assumption.
+      - right. apply IHt2. assumption.
+Qed.
+
 (******************** Substitutions **********************)
 (* Substitution *)
 Definition subst : Set := list (name * term).
@@ -49,6 +109,9 @@ Definition subst : Set := list (name * term).
 Definition empty_subst : subst := [].
 
 Definition singleton_subst (n : name) (t : term) := [(n, t)].
+
+(* Substitution domain *)
+Definition domain (s : subst) : list name := nodup name_eq_dec (map (@fst name term) s).
 
 (* Substitution image *)
 Fixpoint image (s : subst) (n : name) : option term :=
@@ -68,6 +131,24 @@ Fixpoint apply (s : subst) (t : term) : term :=
 Lemma apply_empty: forall (t : term), apply empty_subst t = t.
 Proof.
   induction t; try (simpl; congruence); auto.
+Qed.
+
+(* Free variables in the result of a singleton substitution application *)
+Lemma apply_fv: forall t s n m,  In m (fv_term (apply [(n, s)] t)) -> In m (fv_term s) \/ In m (fv_term t).
+Proof.
+  induction t.
+  * intros. unfold apply in H. unfold image in H. destruct (Nat.eq_dec n0 n).
+    + left. assumption.
+    + right. assumption.
+  * intros. inversion H.
+  * intros. unfold apply in H. fold apply in H.
+    unfold fv_term in H. fold fv_term in H. apply (set_union_elim name_eq_dec) in H. destruct H.
+    + apply IHt1 in H. destruct H.
+      - left. assumption.
+      - right. unfold fv_term. fold fv_term. apply (set_union_intro name_eq_dec). left. assumption.
+    + apply IHt2 in H. destruct H.
+      - left. assumption.
+      - right. unfold fv_term. fold fv_term. apply (set_union_intro name_eq_dec). right. assumption.
 Qed.
 
 (* Composition *)
@@ -100,189 +181,323 @@ Definition more_general (m s : subst) : Prop :=
 (* Unification property *)
 Definition unifier (s : subst) (t1 t2 : term) : Prop := apply s t1 = apply s t2.
 
-Inductive MGU : term -> term -> option subst -> Prop :=
-| MGU_VVEq        : forall n,
-                    MGU (Var n) (Var n) (Some empty_subst)
-| MGU_VVNeq       : forall n1 n2,
-                    n1 <> n2 ->
-                    MGU (Var n1) (Var n2) (Some (singleton_subst n1 (Var n2)))
-| MGU_VCst        : forall n c,
-                    MGU (Var n) (Cst c) (Some (singleton_subst n (Cst c)))
-| MGU_VConOccurs  : forall n c t1 t2,
-                    occurs n (Con c t1 t2) = true ->
-                    MGU (Var n) (Con c t1 t2) None
-| MGU_VConSucc    : forall n c t1 t2,
-                    occurs n (Con c t1 t2) = false ->
-                    MGU (Var n) (Con c t1 t2) (Some (singleton_subst n (Con c t1 t2)))
-| MGU_CstV        : forall n c,
-                    MGU (Cst c) (Var n) (Some (singleton_subst n (Cst c)))
-| MGU_ConVOccurs  : forall n c t1 t2,
-                    occurs n (Con c t1 t2) = true ->
-                    MGU (Con c t1 t2) (Var n) None
-| MGU_ConVSucc    : forall n c t1 t2,
-                    occurs n (Con c t1 t2) = false ->
-                    MGU (Con c t1 t2) (Var n) (Some (singleton_subst n (Con c t1 t2)))
-| MGU_CstCstNeq   : forall c1 c2,
-                    c1 <> c2 ->
-                    MGU (Cst c1) (Cst c2) None
-| MGU_CstCstEq    : forall c,
-                    MGU (Cst c) (Cst c) (Some empty_subst)
-| MGU_ConConNeq   : forall c1 l1 r1 c2 l2 r2,
-                    c1 <> c2 ->
-                    MGU (Con c1 l1 r1) (Con c2 l2 r2) None
-| MGU_ConConEqFL  : forall c l1 r1 l2 r2,
-                    MGU l1 l2 None ->
-                    MGU (Con c l1 r1) (Con c l2 r2) None
-| MGU_ConConEqFR  : forall c l1 r1 l2 r2 sl,
-                    MGU l1 l2 (Some sl) ->
-                    MGU (apply sl r1) (apply sl r2) None ->
-                    MGU (Con c l1 r1) (Con c l2 r2) None
-| MGU_ConConEqSuc : forall c l1 r1 l2 r2 sl sr s,
-                    MGU l1 l2 (Some sl) ->
-                    MGU (apply sl r1) (apply sl r2) (Some sr) ->
-                    s = compose sl sr ->
-                    MGU (Con c l1 r1) (Con c l2 r2) (Some s).
+(* MGU *)
+(* Definition mgu (m : subst) (t1 t2 : term) : Prop :=
+  unifier m t1 t2 /\ forall (s : subst), unifier s t1 t2 -> more_general m s.
+*)
 
-Example test1: MGU (Cst 1)                 (Cst 2)                  None.                           Proof. constructor. intro C. inversion C. Qed.
-Example test2: MGU (Cst 1)                 (Cst 1)                 (Some []).                       Proof. constructor. Qed.
-Example test3: MGU (Var 1)                 (Var 2)                 (Some [(1, Var 2)]).             Proof. constructor. intro C. inversion C. Qed.
-Example test4: MGU (Var 1)                 (Var 1)                 (Some []).                       Proof. constructor. Qed.
-Example test5: MGU (Con 1 (Var 1) (Var 2)) (Con 2 (Var 1) (Var 2))  None.                           Proof. constructor. intro C. inversion C. Qed.
-Example test6: MGU (Con 1 (Var 1) (Var 2)) (Con 1 (Var 1) (Var 2)) (Some []).                       Proof. econstructor. constructor. constructor. reflexivity. Qed.
-Example test7: MGU (Con 1 (Var 1) (Var 1)) (Con 1 (Var 1) (Var 2)) (Some [(1, Var 2)]).             Proof. econstructor. constructor. constructor. intro C. inversion C. reflexivity. Qed.
-Example test8: MGU (Con 1 (Cst 1) (Var 2)) (Con 1 (Var 1) (Cst 2)) (Some [(1, Cst 1); (2, Cst 2)]). Proof. econstructor. constructor. constructor. reflexivity. Qed.
+Inductive unification_step_outcome : Set :=
+| Fail : unification_step_outcome
+| Fine : unification_step_outcome
+| Subst : forall (n: name) (t: term), unification_step_outcome.
 
-Lemma apply_singleton_eq :
-  forall n t, apply (singleton_subst n t) (Var n) = t.
+Definition create (n: name) (t: term) : unification_step_outcome :=
+  if occurs n t then Fail else Subst n t.
+
+(* Find a difference in a couple of terms and try to make a unification step *)
+Fixpoint unification_step (t1 t2 : term) : unification_step_outcome :=
+  match (t1, t2) with
+  | (Cst n1      , Cst n2      ) => if eq_nat_dec n1 n2 then Fine else Fail 
+  | (Con n1 l1 r1, Con n2 l2 r2) => if eq_nat_dec n1 n2
+                                    then
+                                      match unification_step l1 l2 with
+                                      | Fail => Fail
+                                      | Fine => unification_step r1 r2
+                                      | res  => res
+                                      end
+                                    else Fail
+  | (Var n1      , Var n2      ) => if eq_nat_dec n1 n2 then Fine else create n1 t2
+  | (Var n1      , _           ) => create n1 t2
+  | (_           , Var n2      ) => create n2 t1
+  | (_           , _           ) => Fail
+  end.
+
+Definition unification_step_ok t1 t2 n s := unification_step t1 t2 = Subst n s.
+
+Lemma unification_step_fv: forall t1 t2 s n ,
+    unification_step_ok t1 t2 n s -> (forall m, In m (fv_term s) -> In m (fv_term t1) \/ In m (fv_term t2)).
 Proof.
-  intros. simpl. destruct (Nat.eq_dec n n). reflexivity. contradiction.
+  assert (invCr: forall n0 n1 t0 t1, create n0 t0 = Subst n1 t1 -> t0 = t1).
+  { intros. unfold create in H. destruct (occurs n0 t0).
+    - inversion H.
+    - inversion H. reflexivity. }
+  induction t1.
+  * intros. unfold unification_step_ok in H. destruct t2; unfold unification_step in H.
+    + destruct (Nat.eq_dec n n1).
+      - inversion H.
+      - apply invCr in H; subst. right. assumption.
+    + apply invCr in H; subst. right. assumption.
+    + apply invCr in H; subst. right. assumption.
+  * intros. unfold unification_step_ok in H. destruct t2; unfold unification_step in H.
+    + apply invCr in H; subst. left. assumption.
+    + destruct (Nat.eq_dec n n1); inversion H.
+    + inversion H.
+  * intros. unfold unification_step_ok in H. destruct t2; unfold unification_step in H.
+    + apply invCr in H; subst. left. assumption.
+    + inversion H.
+    + fold unification_step in H. destruct (Nat.eq_dec n n1).
+      - destruct (unification_step t1_1 t2_1) eqn:eq.
+        { inversion H. }
+        { unfold unification_step_ok in IHt1_2. apply IHt1_2 with (m := m) in H.
+          - destruct H.
+            + left. unfold fv_term. fold fv_term. apply (set_union_intro name_eq_dec). right. assumption.
+            + right. unfold fv_term. fold fv_term. apply (set_union_intro name_eq_dec). right. assumption.
+          - assumption. }
+        { inversion H; subst. unfold unification_step_ok in IHt1_1.
+          apply IHt1_1 with (m := m) in eq.
+          - destruct eq.
+            + left. unfold fv_term. fold fv_term. apply (set_union_intro name_eq_dec). left. assumption.
+            + right. unfold fv_term. fold fv_term. apply (set_union_intro name_eq_dec). left. assumption.
+          - assumption. }
+      - inversion H.
 Qed.
 
-Lemma apply_singleton_not_occurs :
-  forall n tn t,
-    occurs n t = false -> apply (singleton_subst n tn) t = t.
+Lemma unification_step_subst_wf:
+  forall t1 t2 s n, unification_step_ok t1 t2 n s -> ~ In n (fv_term s).
 Proof.
-  intros n tn t. induction t; simpl.
-  * intros H. apply Nat.eqb_neq in H. destruct (Nat.eq_dec n0 n).
-    + symmetry in e. contradiction.
-    + destruct (Nat.eq_dec n n0).
-      - symmetry in e. contradiction.
-      - reflexivity.
-  * intros _. reflexivity.
-  * intros H. apply Bool.orb_false_elim in H.
-      destruct H. rewrite IHt1; auto; rewrite IHt2; auto.
-Qed.
-
-Lemma mgu_unifies:
-  forall (t1 t2 : term) (s : subst), MGU t1 t2 (Some s) -> unifier s t1 t2.
-Proof.
-  intros. remember (Some s) as r. red. revert s Heqr.
-  induction H; intros ss Heqr; inversion Heqr; clear Heqr; subst.
-  * reflexivity.
-  * rewrite apply_singleton_eq. rewrite apply_singleton_not_occurs.
-    + reflexivity.
-    + simpl. apply Nat.eqb_neq. assumption.
-  * rewrite apply_singleton_eq. reflexivity.
-  * rewrite apply_singleton_eq. rewrite apply_singleton_not_occurs. reflexivity.
-    { assumption. }
-  * rewrite apply_singleton_eq. reflexivity.
-  * rewrite apply_singleton_eq. rewrite apply_singleton_not_occurs. reflexivity.
-    { assumption. }
-  * reflexivity.
-  * simpl. assert (Heql: apply (compose sl sr) l1 = apply (compose sl sr) l2).
-    { rewrite compose_correctness. rewrite compose_correctness. rewrite IHMGU1; reflexivity. }
-    rewrite Heql. assert (Heqr: apply (compose sl sr) r1 = apply (compose sl sr) r2).
-    { rewrite compose_correctness. rewrite compose_correctness. rewrite IHMGU2; reflexivity. }
-    rewrite Heqr. reflexivity.
-Qed.
-
-Lemma mgu_is_most_general:
-  forall (t1 t2 : term) (m : subst),
-    MGU t1 t2 (Some m) -> forall (s : subst), unifier s t1 t2 -> more_general m s.
-Proof.
-  assert (L : forall (n : name) (tn : term) (s : subst),
-      apply s (Var n) = apply s tn ->
-      forall t : term, apply s t = apply s (apply (singleton_subst n tn) t)).
+  intros. assert (exists m t, create m t = Subst n s).
   {
-    intros. induction t.
-    * simpl. destruct (Nat.eq_dec n n0).
-      + rewrite <- H. rewrite e. reflexivity.
-      + reflexivity.
-    * reflexivity.
-    * simpl. congruence.
+    generalize dependent t2. induction t1; intros.
+    * destruct t2; unfold unification_step_ok in H; unfold unification_step in H.
+      + destruct (Nat.eq_dec n0 n1).
+         - inversion H.
+         - eexists. eexists. eapply H.
+      + eexists. eexists. eapply H.
+      + eexists. eexists. eapply H.
+    * destruct t2; unfold unification_step_ok in H; unfold unification_step in H.
+      + eexists. eexists. eapply H.
+      + destruct (Nat.eq_dec n0 n1); inversion H.
+      + inversion H.
+    * destruct t2; unfold unification_step_ok in H; unfold unification_step in H.
+      + eexists. eexists. eapply H.
+      + inversion H.
+      + destruct (Nat.eq_dec n0 n1).
+        - fold unification_step in H. destruct (unification_step t1_1 t2_1) eqn:eq.
+          { inversion H. }
+          { eapply IHt1_2. unfold unification_step_ok. eapply H. }
+          { inversion H; subst. eapply IHt1_1. unfold unification_step_ok.
+            eapply eq. }
+        - inversion H.
   }
-  unfold more_general. unfold unifier. intros t1 t2 m H.
-  remember (Some m) as r. revert m Heqr.
-  induction H; intros m Heqr; inversion Heqr; clear Heqr; subst.
-  * intros. exists s. intros. rewrite <- compose_correctness. reflexivity.
-  * intros. exists s. induction t.
-    + simpl. destruct (Nat.eq_dec n1 n).
-      - rewrite <- H0. rewrite e. reflexivity.
-      - reflexivity.
-    + reflexivity.
-    + simpl. rewrite IHt1. rewrite IHt2. reflexivity.
-  * intros. exists s. apply L. assumption.
-  * intros. exists s. apply L. assumption.
-  * intros. exists s. apply L. symmetry. assumption.
-  * intros. exists s. apply L. symmetry. assumption.
-  * intros. exists s. intros. rewrite apply_empty. reflexivity.
-  * intros. inversion H1. clear H1.
-    apply (IHMGU1 sl eq_refl s) in H3. destruct H3 as [ds H3].
-    rewrite H3 in H4. rewrite H3 in H4.
-    apply (IHMGU2 sr eq_refl ds) in H4. destruct H4 as [dds H4].
-    exists dds. intros. rewrite H3. rewrite H4. rewrite compose_correctness.
-    reflexivity.
+  destruct H0. destruct H0. unfold create in H0. destruct (occurs x x0) eqn:eq.
+  - inversion H0.
+  - inversion H0; subst. intros CH. apply occurs_In in CH. rewrite eq in CH.
+    inversion CH.
 Qed.
 
-Lemma occurs_subst_height: forall s n t,
-  occurs n t = true -> height (apply s (Var n)) <= height (apply s t).
+Lemma unification_step_subst_occurs:
+  forall t1 t2 s n, unification_step_ok t1 t2 n s -> In n (fv_term t1) \/ In n (fv_term t2).
 Proof.
-  intros. induction t.
-  * simpl in H. apply Nat.eqb_eq in H. subst. reflexivity.
-  * inversion H.
-  * simpl in H. apply Bool.orb_true_elim in H. destruct H.
-    + apply IHt1 in e. simpl. apply le_S. eapply le_trans.
-      eassumption. apply Nat.le_max_l.
-    + apply IHt2 in e. simpl. apply le_S. eapply le_trans.
-      eassumption. apply Nat.le_max_r.
+  assert (invCr: forall n0 n1 t0 t1, create n0 t0 = Subst n1 t1 -> n0 = n1).
+  { intros. unfold create in H. destruct (occurs n0 t0).
+    - inversion H.
+    - inversion H. reflexivity. }
+  assert (fvInFv: forall n, In n (fv_term (Var n))).
+  { unfold fv_term. unfold In. left. reflexivity. }
+  induction t1.
+  * intros. unfold unification_step_ok in H. destruct t2; unfold unification_step in H.
+    + destruct (Nat.eq_dec n n1).
+      - inversion H.
+      - apply invCr in H; subst. left. apply fvInFv.
+    + apply invCr in H; subst. left. apply fvInFv.
+    + apply invCr in H; subst. left. apply fvInFv.
+  * intros. unfold unification_step_ok in H. destruct t2; unfold unification_step in H.
+    + apply invCr in H; subst. right. apply fvInFv.
+    + destruct (Nat.eq_dec n n1); inversion H.
+    + inversion H.
+  * intros. unfold unification_step_ok in H. destruct t2; unfold unification_step in H.
+    + apply invCr in H; subst. right. apply fvInFv.
+    + inversion H.
+    + fold unification_step in H. destruct (unification_step t1_1 t2_1) eqn:eq.
+      - destruct (Nat.eq_dec n n1); inversion H.
+      - destruct (Nat.eq_dec n n1).
+        { unfold unification_step_ok in IHt1_2. apply IHt1_2 in H. destruct H.
+          * left. unfold fv_term. fold fv_term. apply (set_union_intro name_eq_dec). right. assumption.
+          * right. unfold fv_term. fold fv_term. apply (set_union_intro name_eq_dec). right. assumption. }
+        inversion H.
+      - destruct (Nat.eq_dec n n1); inversion H; subst.
+        unfold unification_step_ok in IHt1_1. apply IHt1_1 in eq. destruct eq.
+        { left. unfold fv_term. fold fv_term. apply (set_union_intro name_eq_dec). left. assumption. }
+        right. unfold fv_term. fold fv_term. apply (set_union_intro name_eq_dec). left. assumption.
 Qed.
 
-Lemma mgu_non_unifiable:
-  forall (t1 t2 : term),
-    MGU t1 t2 None -> ~(exists (s : subst), unifier s t1 t2).
+Lemma unification_step_subst_elims: forall s t n, In n (fv_term (apply (singleton_subst n s) t)) -> In n (fv_term s).
 Proof.
-  assert (occurs_check_H: forall n c l r,
-    occurs n (Con c l r) = true -> ~(exists (s : subst), apply s (Var n) = apply s (Con c l r))).
-  {
-    intros. intro. destruct H0 as [s H0].
-    assert (height (apply s (Var n)) < height (apply s (Con c l r))).
-    {
-      simpl. apply le_lt_n_Sm. simpl in H.
-      apply Bool.orb_true_elim in H. destruct H.
-      * eapply le_trans.
-        + eapply occurs_subst_height. eassumption.
-        + apply Nat.le_max_l.
-      * eapply le_trans.
-        + eapply occurs_subst_height. eassumption.
-        + apply Nat.le_max_r.
+  intros s t n. unfold singleton_subst. induction t.
+  * unfold apply. unfold image. destruct (Nat.eq_dec n n0).
+    + auto.
+    + unfold fv_term. intros. exfalso. inversion H.
+      - apply n1. symmetry. assumption.
+      - inversion H0.
+  * intros. inversion H.
+  * intros. unfold apply in H. fold apply in H. unfold fv_term in H. fold fv_term in H.
+    apply (set_union_elim name_eq_dec) in H. destruct H; auto.
+Qed.
+
+Lemma lt_size:
+  forall (vs1 vs2 : var_set),
+    NoDup vs1 -> NoDup vs2 -> incl vs1 vs2 -> (exists n, In n vs2 /\ ~ (In n vs1)) -> var_set_size vs1 < var_set_size vs2.
+Proof.
+  intros. destruct H2. destruct H2. apply in_split in H2.
+  destruct H2. destruct H2. subst.
+  unfold var_set_size. rewrite app_length. simpl.
+  assert (length vs1 <= length (x0 ++ x1)).
+  { apply NoDup_incl_length.
+    * assumption.
+    * unfold incl. intros. assert (H2_copy := H2).
+      apply H1 in H2. apply in_app_or in H2. destruct H2.
+      + apply in_or_app. left. assumption.
+      + inversion H2.
+        - exfalso. apply H3. congruence.
+        - apply in_or_app. right. assumption. }
+  rewrite app_length in H2. omega.
+Qed.
+
+Lemma unification_step_decreases_fv:
+  forall t1 t2 s n,
+    unification_step_ok t1 t2 n s ->
+    var_set_size (var_set_union (fv_term (apply (singleton_subst n s) t1)) (fv_term (apply [(n, s)] t2))) < var_set_size (var_set_union (fv_term t1) (fv_term t2)).
+Proof.
+  intros t1 t2 s n USok.
+  apply lt_size; try apply union_NoDup.
+  * apply set_union_nodup; apply fv_term_nodup.
+  * apply set_union_nodup; apply fv_term_nodup.
+  * intros n0 InH. apply (set_union_elim name_eq_dec) in InH. inversion_clear InH.
+    + apply apply_fv in H. inversion_clear H.
+      - apply unification_step_fv with (m:=n0) in USok.
+        { apply (set_union_intro name_eq_dec). assumption. }
+        assumption.
+      - apply (set_union_intro name_eq_dec). left. assumption.
+    + apply apply_fv in H. inversion_clear H.
+      - apply unification_step_fv with (m:=n0) in USok.
+        { apply (set_union_intro name_eq_dec). assumption. }
+        assumption.
+      - apply (set_union_intro name_eq_dec). right. assumption.
+  * exists n. split.
+    + apply unification_step_subst_occurs in USok. apply (set_union_intro name_eq_dec). assumption.
+    + unfold not. intro H. apply (set_union_elim name_eq_dec) in H. inversion_clear H as [H0 | H0];
+      apply unification_step_subst_elims in H0;
+      apply unification_step_subst_wf in USok; auto.
+Qed.
+
+Definition terms := (term * term)%type.
+
+Definition fvOrder (t : terms) := length (var_set_union (fv_term (fst t)) (fv_term (snd t))).
+
+Definition fvOrderRel (t p : terms) := fvOrder t < fvOrder p.
+
+Hint Constructors Acc.
+
+Theorem fvOrder_wf: well_founded fvOrderRel.
+Proof.
+  assert (fvOrder_wf': forall (size: nat) (t: terms), fvOrder t < size -> Acc fvOrderRel t).
+    {unfold fvOrderRel. induction size.
+     * intros. inversion H.
+     * intros. constructor. intros. apply IHsize. omega.
     }
-    rewrite H0 in H1. eapply Nat.lt_irrefl. eassumption.
+  red; intro; eapply fvOrder_wf'; eauto.
+Defined.
+
+Inductive unify : term -> term -> option subst -> Prop :=
+| unify_Fail : forall t1 t2, unification_step t1 t2 = Fail -> unify t1 t2 None
+| unify_Fine : forall t1 t2, unification_step t1 t2 = Fine -> unify t1 t2 (Some empty_subst)
+| unify_SubstNone : forall t1 t2 n s, unification_step t1 t2 = Subst n s ->
+                                      unify (apply (singleton_subst n s) t1) (apply (singleton_subst n s) t2) None ->
+                                      unify t1 t2 None
+| unify_SubstSome : forall t1 t2 n s r sr, unification_step t1 t2 = Subst n s ->
+                                           unify (apply (singleton_subst n s) t1) (apply (singleton_subst n s) t2) (Some r) ->
+                                           sr = compose (singleton_subst n s) r ->
+                                           unify t1 t2 (Some sr).
+
+Example test1: unify (Cst 1)                 (Cst 2)                 None.                            Proof. repeat econstructor. Qed.
+Example test2: unify (Cst 1)                 (Cst 1)                 (Some []).                       Proof. repeat econstructor. Qed.
+Example test3: unify (Var 1)                 (Var 2)                 (Some [(1, Var 2)]).             Proof. repeat econstructor. Qed.
+Example test4: unify (Var 1)                 (Var 1)                 (Some []).                       Proof. repeat econstructor. Qed.
+Example test5: unify (Con 1 (Var 1) (Var 2)) (Con 2 (Var 1) (Var 2)) None.                            Proof. repeat econstructor. Qed.
+Example test6: unify (Con 1 (Var 1) (Var 2)) (Con 1 (Var 1) (Var 2)) (Some []).                       Proof. repeat econstructor. Qed.
+Example test7: unify (Con 1 (Var 1) (Var 1)) (Con 1 (Var 1) (Var 2)) (Some [(1, Var 2)]).             Proof. repeat econstructor. Qed.
+Example test8: unify (Con 1 (Cst 1) (Var 2)) (Con 1 (Var 1) (Cst 2)) (Some [(1, Cst 1); (2, Cst 2)]). Proof. econstructor. econstructor. eapply unify_SubstSome. econstructor. econstructor. econstructor. econstructor. econstructor. Qed.
+
+Lemma unify_works : forall t1 t2, exists r, unify t1 t2 r.
+Proof.
+  intros t1 t2.
+  remember (fun p => exists r : option subst, unify (fst p) (snd p) r) as P.
+  assert (P (t1, t2)).
+  {
+    apply well_founded_induction with (R := fvOrderRel).
+    * apply fvOrder_wf.
+    * intros. subst. clear t1 t2. destruct x as [t1 t2]. simpl.
+      destruct (unification_step t1 t2) eqn:eq.
+      + exists None. constructor. assumption.
+      + exists (Some empty_subst). constructor. assumption.
+      + specialize (H (apply (singleton_subst n t) t1, apply (singleton_subst n t) t2)).
+        assert (fvOr : fvOrderRel (apply (singleton_subst n t) t1, apply (singleton_subst n t) t2) (t1, t2)).
+        { apply unification_step_decreases_fv. assumption. }
+        specialize (H fvOr). destruct H. destruct x.
+        - eexists. eapply unify_SubstSome.
+          { eassumption. }
+          { eassumption. }
+          { reflexivity. }
+        - exists None. eapply unify_SubstNone.
+          { eassumption. }
+          { eassumption. }
   }
-  intros. remember None as r. unfold unifier.
-  induction H; inversion Heqr; clear Heqr; subst.
-  * apply occurs_check_H. assumption.
-  * intro. destruct H0 as [s H0]. eapply occurs_check_H.
-    eassumption. exists s. symmetry. assumption.
-  * intro. destruct H0 as [s H0]. inversion H0. contradiction.
-  * intro. destruct H0 as [s H0]. inversion H0. contradiction.
-  * intro. destruct H0 as [s H0]. apply IHMGU.
-    + reflexivity.
-    + exists s. inversion H0. reflexivity.
-  * intro. destruct H1 as [s H1]. apply IHMGU2.
-    + reflexivity.
-    + inversion H1. eapply mgu_is_most_general in H.
-      2: { eassumption. }
-      { destruct H as [ds H]. exists ds.
-        rewrite <- H. rewrite <- H. assumption. }
+  subst. assumption.
 Qed.
 
+Lemma fine_step_equal_terms :
+  forall t1 t2,
+    unification_step t1 t2 = Fine -> t1 = t2.
+Proof.
+  assert (createFine : forall n t, create n t <> Fine).
+  { unfold create. intros n t C. destruct (occurs n t); inversion C. }
+  induction t1; induction t2; intro us_eq; inversion us_eq; clear us_eq; subst.
+  - destruct (Nat.eq_dec n n0).
+    { congruence. }
+    { apply createFine in H0. contradiction. }
+  - apply createFine in H0. contradiction.
+  - destruct (Nat.eq_dec n n0).
+    { congruence. }
+    { inversion H0. }
+  - apply createFine in H0. contradiction.
+  - destruct (Nat.eq_dec n n0).
+    { subst. destruct (unification_step t1_1 t2_1) eqn:eq; inversion H0.
+      apply IHt1_1 in eq. apply IHt1_2 in H0. congruence. }
+    { inversion H0. }
+Qed.
+
+
+Lemma unify_unifies:
+  forall t1 t2 s,
+    unify t1 t2 (Some s) -> unifier s t1 t2.
+Proof.
+  intros t1 t2. remember (fun p => forall s : subst,
+      unify (fst p) (snd p) (Some s) -> unifier s (fst p) (snd p)).
+  assert (P (t1, t2)).
+  {
+    apply well_founded_induction with (R := fvOrderRel).
+    * apply fvOrder_wf.
+    * intros. subst. clear t1 t2. destruct x as [t1 t2]. simpl.
+      intros. inversion H0; subst; clear H0.
+      + unfold unifier. rewrite apply_empty. rewrite apply_empty.
+        apply fine_step_equal_terms. assumption.
+      + assert (fvOr : fvOrderRel (apply (singleton_subst n s0) t1, apply (singleton_subst n s0) t2) (t1, t2)).
+        { apply unification_step_decreases_fv. assumption. }
+        eapply H in fvOr.
+        2: { eassumption. }
+        { unfold unifier. rewrite compose_correctness. rewrite compose_correctness.
+          assumption. }
+  }
+  subst. assumption.
+Qed.
+
+Lemma unify_most_general :
+  forall (t1 t2 : term) (m : subst),
+    unify t1 t2 (Some m) ->
+    forall (s : subst), unifier s t1 t2 -> more_general m s.
+Proof. admit. Admitted.
+
+Lemma non_unifiable_not_unify:
+  forall (t1 t2 : term),
+    unify t1 t2 None -> forall s,  ~ (unifier s t1 t2).
+Proof. admit. Admitted.
